Improve error checking

Source/DafnyCore/Resolver/DetectUnsoundFunctionReferencesVisitor.cs
@@ -2,9 +2,18 @@ using System.Diagnostics.Contracts;
 
 namespace Microsoft.Dafny;
 
+/// <summary>
+/// This class checks three conditions:
+///   0. A function declared with `reads **` is never used naked (i.e., every use of it is applied to arguments)
+///   1. A function is never used naked in its own definition (that is, anywhere in the definition of itself or of a mutually recursive callable)
+///   2. The decreases clause of a function never makes any recursive or mutually recursive calls to the function itself
+/// </summary>
 class DetectUnsoundFunctionReferencesVisitor : ResolverBottomUpVisitor {
   private readonly ICallable context;
-  private bool doDecreasesChecks;
+
+  private enum Checks { Check0, Check0And1, Check2 }
+  private Checks whichChecks;
+
   private DetectUnsoundFunctionReferencesVisitor(ModuleResolver resolver, ICallable context)
     : base(resolver) {
     Contract.Requires(resolver != null);
@@ -14,31 +23,42 @@ class DetectUnsoundFunctionReferencesVisitor : ResolverBottomUpVisitor {
 
   public static void Check(ICallable callable, ModuleResolver resolver) {
     var visitor = new DetectUnsoundFunctionReferencesVisitor(resolver, callable);
-    visitor.doDecreasesChecks = false;
     if (callable is Function function) {
+      visitor.whichChecks = Checks.Check0And1;
       visitor.VisitFunctionWithoutByMethod(function);
+      if (function.ByMethodBody != null) {
+        // don't do check 1 in the by-method clause, since the by-method sits strictly above its function in the call graph
+        visitor.whichChecks = Checks.Check0;
+        visitor.Visit(function.ByMethodBody);
+      }
+      // visit the "decreases" clause again, this time performing check 2
+      visitor.whichChecks = Checks.Check2;
+      visitor.Visit(callable.Decreases.Expressions);
+
     } else {
+      // for the non-function, just performs checks 0 and 1
+      visitor.whichChecks = Checks.Check0And1;
       visitor.Visit(callable);
     }
-    visitor.doDecreasesChecks = true;
-    visitor.Visit(callable.Decreases.Expressions);
   }
 
   protected override void VisitOneExpr(Expression expr) {
     if (expr is MemberSelectExpr { Member: Function fn }) {
-      if (fn.ReadsDoubleStar) {
+      // Check 0
+      if (whichChecks is Checks.Check0 or Checks.Check0And1 && fn.ReadsDoubleStar) {
         resolver.reporter.Error(MessageSource.Resolver, expr.Origin,
           "a function declared with 'reads **' can only be used if applied to arguments");
       }
 
-      if (!doDecreasesChecks && ModuleDefinition.InSameSCC(context, fn)) {
+      // Check 1
+      if (whichChecks == Checks.Check0And1 && ModuleDefinition.InSameSCC(context, fn)) {
         resolver.reporter.Error(MessageSource.Resolver, expr.Origin,
           "cannot use naked function in recursive setting. Possible solution: eta expansion.");
       }
-
     }
 
-    if (doDecreasesChecks && expr is FunctionCallExpr callExpr && ModuleDefinition.InSameSCC(context, callExpr.Function)) {
+    // Check 2
+    if (whichChecks == Checks.Check2 && expr is FunctionCallExpr callExpr && ModuleDefinition.InSameSCC(context, callExpr.Function)) {
       string msg;
       if (context == callExpr.Function) {
         msg = "a decreases clause is not allowed to call the enclosing function";
